thys/Infinitary_Lambda_Calculus/ILC_affine.thy
@@ -21,9 +21,8 @@ inductive affine  :: "itrm \<Rightarrow> bool" where
  \<Longrightarrow>
  affine (iApp e1 es2)"
 
-binder_inductive affine
-
-  (*unfolding isPerm_def induct_rulify_fallback
+binder_inductive (no_auto_equiv, no_auto_refresh) affine
+  unfolding isPerm_def induct_rulify_fallback
   subgoal for R B \<sigma> t
     apply(elim disjE)
     subgoal apply(rule disjI3_1)
@@ -51,7 +50,7 @@ binder_inductive affine
         done
       done
     done
-  done*)
+  done
   subgoal premises prems for R B t
     using prems(2-)
      apply safe
