thys/Untyped_Lambda_Calculus/LC_Parallel_Beta.thy
@@ -15,17 +15,17 @@ inductive pstep :: "trm \<Rightarrow> trm \<Rightarrow> bool" where
 | Xi: "pstep e e' \<Longrightarrow> pstep (Lam x e) (Lam x e')"
 | PBeta: "pstep e1 e1' \<Longrightarrow> pstep e2 e2' \<Longrightarrow> pstep (App (Lam x e1) e2) (tvsubst (Var(x:=e2')) e1')"
 
-binder_inductive pstep
-  subgoal premises prems for R B t1 t2
-    by (tactic \<open>refreshability_tac false
-      [@{term "FFVars :: trm \<Rightarrow> var set"}, @{term "FFVars :: trm \<Rightarrow> var set"}]
+binder_inductive (no_auto_refresh) pstep
+ subgoal premises prems for R B t1 t2
+     by (tactic \<open>refreshability_tac false
+       [@{term "FFVars :: trm \<Rightarrow> var set"}, @{term "FFVars :: trm \<Rightarrow> var set"}]
       [@{term "rrename :: (var \<Rightarrow> var) \<Rightarrow> trm \<Rightarrow> trm"}, @{term "(\<lambda>f x. f x) :: (var \<Rightarrow> var) \<Rightarrow> var \<Rightarrow> var"}]
       [NONE, NONE, SOME [SOME 0, SOME 0, SOME 1], SOME [SOME 0, SOME 0, NONE, NONE, SOME 1]]
       @{thm prems(3)} @{thm prems(2)} @{thms }
       @{thms emp_bound singl_bound term.Un_bound term.card_of_FFVars_bounds infinite}
       @{thms Lam_inject} @{thms Lam_eq_tvsubst term.rrename_cong_ids[symmetric]}
       @{thms id_on_antimono} @{context}\<close>)
-  done
+ done
 
 thm pstep.strong_induct
 thm pstep.equiv
